Add builtin eval

Bar.lean
@@ -1,13 +1,26 @@
-
 def hello := "world"
 open String
 open Nat
 open Int
 open List
 
-structure Builtin where
-  function: Nat
+-- Term and Program Structures
+def Name := String
 deriving Repr
+
+inductive Function where
+  | addInteger : Function
+  | subtractInteger : Function
+deriving Repr
+
+structure Builtin where
+  function: Function
+deriving Repr
+
+def builtin_arity (function: Function): Nat × Nat :=
+  match function with
+  | .addInteger => (0, 2)
+  | .subtractInteger => (0, 2)
 
 inductive Term where
   | var (x : String) : Term
@@ -25,6 +38,7 @@ structure Program where
  m: Term
 deriving Repr
 
+-- Value Structures
 mutual
 inductive Value where
   | vCon (c : Int) : Value
@@ -40,13 +54,45 @@ inductive BuiltinValue where
 deriving Repr
 end
 
+-- Partial Builtin functions
+def builtin_name (b: BuiltinValue): Function :=
+  match b with
+    | .builtin b => b.function
+    | .app b _ => builtin_name b
+    | .force b => builtin_name b
+
+def force_size (b: BuiltinValue): Nat :=
+  match b with
+    | .force b => (force_size b) + 1
+    | .app b _ => (force_size b)
+    | _ => 0
+
+def builtin_args (b: BuiltinValue): List Value :=
+  match b with
+    | .builtin _ => []
+    | .app b v => (builtin_args b) ++ [v]
+    | .force _ => []
+
+def builtin_size (b: BuiltinValue): Nat × Nat :=
+  match b with
+    | .builtin _ => (0, 0)
+    | .app _ _ => (force_size b, List.length (builtin_args b))
+    | .force _ => (force_size b, 0)
+
+def not_all_args_applied (args: Nat × Nat) (arity: Nat × Nat): Prop :=
+  let (forces, applies) := args
+  let (forces_arity, apply_arity) := arity
+  applies < apply_arity || forces < forces_arity
+
+
+-- Term Reduction
+
 inductive Frame where
   | force : Frame
   | leftAppTerm (m : Term) (p : List (String × Value)) : Frame
   | leftAppValue (v : Value) : Frame
   | rightApp (v : Value) : Frame
 deriving Repr
-
 
 def Stack := List Frame
 deriving Repr
@@ -59,56 +105,100 @@ inductive State where
 deriving Repr
 
 
-def lookup_var (e: List (String × Value)) (x: String) : Option Value :=
+def Environment := List (String × Value)
+
+def lookup_var (e: Environment) (x: String): Option Value :=
   match e with
   | []  => none
   | (y, v) :: e => if x == y then some v else lookup_var e x
 
+
+theorem args_length_is_size {b}: List.length (builtin_args b) = (builtin_size b).snd := by
+  cases b with
+  | builtin a =>
+    rw [builtin_args, builtin_size]
+    rfl
+  | app a v =>
+    rw [builtin_args, builtin_size]
+    simp [builtin_args]
+  | force a =>
+    simp [builtin_args, builtin_size]
+
+theorem args_length_is_arity {b} (h: builtin_size b = builtin_arity (builtin_name b)) :
+  List.length (builtin_args b) = (builtin_arity (builtin_name b)).snd := by
+    have h': List.length (builtin_args b) = (builtin_size b).snd := by
+      apply args_length_is_size
+    have h'': (builtin_arity (builtin_name b)).snd = (builtin_size b).snd := by
+      simp [h]
+    simp [h', h'']
+
+
+
+def eval_builtin (s: Stack) (b: BuiltinValue) (h: builtin_size b = builtin_arity (builtin_name b)) : State :=
+  let args := builtin_args b
+  have j: 1 < List.length args := by
+    simp [args_length_is_arity, h, builtin_arity]
+    cases builtin_name b with
+      | _ => simp
+
+   have jj: 0 < List.length args := by
+    simp [args_length_is_arity, h, builtin_arity]
+    cases builtin_name b with
+      | _ => simp
+
+  match (builtin_name b) with
+    | Function.addInteger => match (args[0]'jj, args[1]'j) with
+      | (Value.vCon l, Value.vCon r) =>
+        State.ret (Value.vCon (l + r)) s
+      | (_, _) => State.error
+
+    | Function.subtractInteger => match (args[0]'jj, args[1]'j) with
+      | (Value.vCon l, Value.vCon r) =>
+        State.ret (Value.vCon (l - r)) s
+      | (_, _) => State.error
+
+
+
+
+
 inductive small_step : State -> State -> Prop
-  | seq {s s' s''} (h: small_step s s') (h': small_step s' s''):
-    small_step s s''
+  | seq {s s' s''} (h: small_step s s') (h': small_step s' s''): small_step s s''
+
   | computeLookup {x p s} (h: lookup_var p x = some v): small_step (State.compute (Term.var x) p s) (State.ret v s)
+
   | computeConstant {c p s} : small_step (State.compute (Term.con c) p s) (State.ret (Value.vCon c) s)
+
   | computeLambda {x m p s} : small_step (State.compute (Term.lam x m) p s) (State.ret (Value.vLam x m p) s)
+
   | computeDelay {m p s} : small_step (State.compute (Term.delay m) p s) (State.ret (Value.vDelay m p) s)
+
   | computeForce {m p s} : small_step (State.compute (Term.force m) p s) (State.compute m p (Frame.force :: s))
+
   | computeApp {m n p s} : small_step (State.compute (Term.app m n) p s) (State.compute m p (Frame.leftAppTerm n p :: s))
+
   | computeBuiltin {b p s} : small_step (State.compute (Term.builtin b) p s) (State.ret (Value.vBuiltin (BuiltinValue.builtin b)) s)
+
   | computeError {p s} : small_step (State.compute Term.error p s) State.error
-  | ret {v s} : small_step (State.ret v s) (State.halt v)
+
+  | ret {v} : small_step (State.ret v []) (State.halt v)
+
   | retLeftAppTerm {m p v s} : small_step (State.ret v (Frame.leftAppTerm m p :: s)) (State.compute m p (Frame.rightApp v :: s))
+
   | retRightApp {x m p v s} : small_step (State.ret v (Frame.rightApp (Value.vLam x m p) :: s)) (State.compute m ((x, v) :: p) s)
+
   | retLeftAppValue {x m p v s} : small_step (State.ret (Value.vLam x m p) (Frame.leftAppValue v :: s)) (State.compute m ((x, v) :: p) s)
-  | retRightAppBuiltin {b v s} : small_step (State.ret v (Frame.rightApp (Value.vBuiltin b) :: s)) (State.ret (Value.vBuiltin (BuiltinValue.app b v)) s)
-  | retLeftAppValueBuiltin {b v s} : small_step (State.ret (Value.vBuiltin b) (Frame.leftAppValue v :: s)) (State.ret (Value.vBuiltin (BuiltinValue.app b v)) s)
-  | retDelay {m p s} : small_step (State.ret (Value.vDelay m p) (Frame.force :: s)) (State.compute m p s)
-  | retBuiltin {b s} : small_step (State.ret (Value.vBuiltin b) (Frame.force :: s)) (State.ret (Value.vBuiltin (BuiltinValue.force b)) s)
+
+  | retRightAppBuiltin {b v s} (h: not_all_args_applied (builtin_size b) (builtin_arity (builtin_name b))) : small_step (State.ret v (Frame.rightApp (Value.vBuiltin b) :: s)) (State.ret (Value.vBuiltin (BuiltinValue.app b v)) s)
+
+  | retLeftAppValueBuiltin {b v s} (h: not_all_args_applied (builtin_size b) (builtin_arity (builtin_name b))) : small_step (State.ret (Value.vBuiltin b) (Frame.leftAppValue v :: s)) (State.ret (Value.vBuiltin (BuiltinValue.app b v)) s)
+
+  | BuiltinEval {b s} (h: builtin_size b = builtin_arity (builtin_name b)) (h': eval_builtin s b h = s' ) : small_step (State.ret (Value.vBuiltin b) s) s'
+
+  | retForceDelay {m p s} : small_step (State.ret (Value.vDelay m p) (Frame.force :: s)) (State.compute m p s)
+
+  | retForceBuiltin {b s} : small_step (State.ret (Value.vBuiltin b) (Frame.force :: s)) (State.ret (Value.vBuiltin (BuiltinValue.force b)) s)
+
   | catchAll {s} : small_step s State.error
-
-  -- inductive small_step : (Instruction × State) -> (Instruction × State) -> Prop
-  -- | seq {m m' m'' s s' s''} (h: small_step (m, s) (m', s')) (h': small_step (m', s') (m'', s'')):
-  --   small_step (m, s) (m'', s'')
-
-  -- | computeLookup {v x p s} (h: lookup_var p x = some v):
-  --   small_step (Instruction.term (Term.var x), State.compute p s) (Instruction.value v, State.ret s)
-
-  -- | computeConstant {c p s} : small_step (Instruction.term (Term.con c) ,State.compute p s) (Instruction.value (Value.vCon c), State.ret s)
-  -- | computeLambda {x m p s} : small_step (Instruction.term (Term.lam x m), State.compute p s) (Instruction.value (Value.vLam x m p), State.ret s)
-  -- | computeDelay {m p s} : small_step (Instruction.term (Term.delay m), State.compute p s) (Instruction.value (Value.vDelay m p), State.ret s)
-  -- | computeForce {m p s} : small_step (Instruction.term (Term.force m), State.compute p s) (Instruction.term m, State.compute p (Frame.force :: s))
-  -- | computeApp {m n p s} : small_step (Instruction.term (Term.app m n), State.compute p s) (Instruction.term m, State.compute p (Frame.leftAppTerm n p :: s))
-  -- | computeBuiltin {b p s} : small_step (Instruction.term (Term.builtin b), State.compute  p s) (Instruction.value (Value.vBuiltin (BuiltinValue.builtin b)), State.ret s)
-  -- | computeError {p s} : small_step (Instruction.term Term.error, State.compute p s) (Instruction.term Term.error, State.error)
-  -- | ret {v} : small_step (Instruction.value v, State.ret []) (Instruction.value v, State.halt)
-  -- | retLeftAppTerm {m p v s} : small_step (Instruction.value v, State.ret (Frame.leftAppTerm m p :: s)) (Instruction.term m, State.compute p (Frame.rightApp v :: s))
-  -- | retRightApp {x m p v s} : small_step (Instruction.value v, State.ret (Frame.rightApp (Value.vLam x m p) :: s)) (Instruction.term m, State.compute ((x, v) :: p) s)
-  -- | retLeftAppValue {x m p v s} : small_step (Instruction.value (Value.vLam x m p), State.ret (Frame.leftAppValue v :: s)) (Instruction.term m, State.compute ((x, v) :: p) s)
-  -- | retRightAppBuiltin {b v s} : small_step (Instruction.value v, State.ret (Frame.rightApp (Value.vBuiltin b) :: s)) (Instruction.value (Value.vBuiltin (BuiltinValue.app b v)), State.ret s)
-  -- | retLeftAppValueBuiltin {b v s} : small_step (Instruction.value (Value.vBuiltin b), State.ret  (Frame.leftAppValue v :: s)) (Instruction.value (Value.vBuiltin (BuiltinValue.app b v)), State.ret s)
-  -- -- TODO: Eval builtins
-  -- | retDelay {m p s} : small_step (Instruction.value (Value.vDelay m p), State.ret (Frame.force :: s)) (Instruction.term m, State.compute p s)
-  -- | retBuiltin {b s} : small_step (Instruction.value (Value.vBuiltin b), State.ret (Frame.force :: s)) (Instruction.value (Value.vBuiltin (BuiltinValue.force b)), State.ret s)
-  -- | catchAll {m s} : small_step (m, s) ((Instruction.term Term.error), State.error)
 
 
 infix: 90 "⟶" => small_step
@@ -129,7 +219,7 @@ theorem frame_force_delay_just_term
         apply small_step.computeDelay
     have h'': (State.ret (Value.vDelay m p) (Frame.force :: s)) ⟶
       (State.compute m p s) := by
-        apply small_step.retDelay
+        apply small_step.retForceDelay
     exact small_step.seq h' h''
 
 theorem forcing
@@ -151,7 +241,7 @@ theorem force_delay_just_term
         apply small_step.computeDelay
     have h'': (State.ret (Value.vDelay m p) (Frame.force :: s)) ⟶
       (State.compute m p s) := by
-        apply small_step.retDelay
+        apply small_step.retForceDelay
     exact small_step.seq (small_step.seq h h') h''
 
 theorem double_force_term
@@ -213,7 +303,7 @@ theorem forces3
   {m p s}:
   (State.compute (Term.force (Term.force (Term.force (Term.delay (Term.delay (Term.delay m)))))) p s) ⟶
   (State.compute m p s) := by
-    repeat (first | apply small_step.computeForce | apply small_step.computeDelay | apply small_step.retDelay | apply small_step.seq)
+    repeat (first | apply small_step.computeForce | apply small_step.computeDelay | apply small_step.retForceDelay | apply small_step.seq)
 
 
 
@@ -240,8 +330,7 @@ theorem lam_apply_var_is_applied_term
               case h =>
                 apply small_step.computeLookup;
                 case h =>
-                  rw [lookup_var]
-                  simp
+                  simp [lookup_var]
                   rfl
               case h' => exact small_step.ret
 
@@ -254,4 +343,14 @@ theorem lam_apply_var_is_applied_term2
   {x p}:
   (State.compute (Term.app (Term.lam x (Term.var x)) (Term.con 5)) p []) ⟶
   (State.halt (Value.vCon 5)) := by
-    repeat (first | apply small_step.computeApp | apply small_step.computeLambda | apply small_step.retLeftAppTerm | apply small_step.computeConstant | apply small_step.retRightApp | apply small_step.computeLookup | apply small_step.ret | apply small_step.seq)
+    repeat (first
+      | apply small_step.computeApp
+      | apply small_step.computeLambda
+      | apply small_step.retLeftAppTerm
+      | apply small_step.computeConstant
+      | apply small_step.retRightApp
+      | apply small_step.computeLookup
+      | simp [lookup_var]
+        rfl
+      | apply small_step.ret
+      | apply small_step.seq)
